internal CF generator: Replace [Wpgen_let_trm_cont] with [Wpgen_let_trm].
- Similar to replacing [Wpgen_seq_cont] with [Wpgen_seq].
- [Wpgen_let_trm_cont] is completely removed (def is commented out).

lib/coq/WPLifted.v
@@ -354,9 +354,9 @@ Proof using. introv HH M1. apply MkStruct_erase. xchanges* HH. Qed.
 (* ** Definition of CF blocks for the internal generator -- DEPRECATED? *)
 
 
-Definition Wpgen_let_trm_cont (F1:Formula) A1 {EA1:Enc A1} (F2of:A1->Formula) : Formula :=
-  MkStruct (fun A (EA:Enc A) Q =>
-    ^F1 (fun (X:A1) => ^(F2of X) Q)).
+(* Definition Wpgen_let_trm_cont (F1:Formula) A1 {EA1:Enc A1} (F2of:A1->Formula) : Formula := *)
+(*   MkStruct (fun A (EA:Enc A) Q => *)
+(*     ^F1 (fun (X:A1) => ^(F2of X) Q)). *)
 
 (* Definition Wpgen_seq_cont (F1 F2:Formula) : Formula := *)
 (*   MkStruct (fun A (EA:Enc A) Q => *)
@@ -382,12 +382,12 @@ Definition Wpaux_getval Wpgen (E:ctx) (t1:trm) (F2of:val->Formula) : Formula :=
 
 Definition Wpaux_getval_typed Wpgen (E:ctx) (t1:trm) `{EA1:Enc A1} (F2of:A1->Formula) : Formula :=
   match t1 with
-  | trm_val v => Wptag (Wpgen_let_trm_cont (Wptag (Wpgen_val_unlifted v)) F2of)
+  | trm_val v => Wptag (Wpgen_let_trm (Wptag (Wpgen_val_unlifted v)) F2of)
   | trm_var x => match Ctx.lookup x E with
-                 | Some v => Wptag (Wpgen_let_trm_cont (Wptag (Wpgen_val_unlifted v)) F2of)
+                 | Some v => Wptag (Wpgen_let_trm (Wptag (Wpgen_val_unlifted v)) F2of)
                  | None => Wptag (Wpgen_fail)
                  end
-  | _ => Wptag (Wpgen_let_trm_cont (Wpgen E t1) F2of)
+  | _ => Wptag (Wpgen_let_trm (Wpgen E t1) F2of)
   end.
 
 Definition Wpaux_constr Wpgen (E:ctx) (id:idconstr) : list val -> list trm -> Formula :=
@@ -415,7 +415,7 @@ Definition Wpaux_var (E:ctx) (x:var) : Formula :=
   end.
 
 Definition Wpaux_if_trm (F0 F1 F2:Formula) : Formula :=
-  Wptag (Wpgen_let_trm_cont F0 (fun (b:bool) => Wptag (Wpgen_if b F1 F2))).
+  Wptag (Wpgen_let_trm F0 (fun (b:bool) => Wptag (Wpgen_if b F1 F2))).
 
 Definition Wpgen_while (F1 F2:Formula) : Formula :=
   MkStruct (Wptag (FormulaCast (fun (Q:unit->hprop) =>
@@ -695,9 +695,8 @@ Lemma Wpgen_sound_seq: forall (F1 F2: Formula) E t1 t2,
   F2 ====> Wpsubst E t2 ->
   Wpgen_seq F1 F2 ====> Wpsubst E (trm_seq t1 t2).
 Proof.
-  introv M1 M2; intros A EA. applys qimpl_Wp_of_Triple; intros Q. remove_MkStruct.
-  apply Triple_hexists; intros Q1.
-  rewrite hstar_comm; apply Triple_hpure; intros M3.
+  introv M1 M2. intros A EA. applys qimpl_Wp_of_Triple. intros Q. remove_MkStruct.
+  apply Triple_hexists; intros Q1. rewrite hstar_comm; apply Triple_hpure; intros M3.
   simpl. applys Triple_seq.
   { rewrite Triple_eq_himpl_Wp. applys M1. }
   { rewrite Triple_eq_himpl_Wp. xchange M3. applys M2. }
@@ -716,30 +715,62 @@ Proof using.
     unfold Subst1. rewrite <- isubst_add_eq_subst1_isubst. applys* M2. }
 Qed.
 
+(* Lemma Wpgen_sound_let_typed : forall (F1:Formula) `{EA1:Enc A1} (F2of:A1->Formula) E (x:var) t1 t2, *)
+(*   F1 ====> Wpsubst E t1 -> *)
+(*   (forall (X:A1), F2of X ====> Wpsubst (Ctx.add x (enc X) E) t2) -> *)
+(*   Wpgen_let_trm_cont F1 F2of ====> Wpsubst E (trm_let x t1 t2). *)
+(* Proof using. *)
+(*   Opaque Ctx.rem. *)
+(*   introv M1 M2. intros A EA. applys qimpl_Wp_of_Triple. intros Q. *)
+(*   remove_MkStruct. xtpull. simpl. applys Triple_let EA1. *)
+(*   (* --LATER: typeclass should not be resolved arbitrarily to EA if EA1 is not provided *) *)
+(*   { rewrite Triple_eq_himpl_Wp. applys* M1. } *)
+(*   { intros X. rewrite Triple_eq_himpl_Wp. *)
+(*     unfold Subst1. rewrite <- isubst_add_eq_subst1_isubst. applys* M2. } *)
+(* Qed. *)
+
+(** Note: Similar to [Wpgen_seq] and [Wpgen_seq_cont], [Wpgen_let_trm_cont] is
+    stronger than [Wpgen_let_trm], but [Wpgen_let_trm] is strong enough to prove
+    soundness. *)
 Lemma Wpgen_sound_let_typed : forall (F1:Formula) `{EA1:Enc A1} (F2of:A1->Formula) E (x:var) t1 t2,
   F1 ====> Wpsubst E t1 ->
   (forall (X:A1), F2of X ====> Wpsubst (Ctx.add x (enc X) E) t2) ->
-  Wpgen_let_trm_cont F1 F2of ====> Wpsubst E (trm_let x t1 t2).
+  Wpgen_let_trm F1 F2of ====> Wpsubst E (trm_let x t1 t2).
 Proof using.
   Opaque Ctx.rem.
-  introv M1 M2. intros A EA. applys qimpl_Wp_of_Triple. intros Q.
-  remove_MkStruct. xtpull. simpl. applys Triple_let EA1.
+  introv M1 M2. intros A EA. applys qimpl_Wp_of_Triple. intros Q. remove_MkStruct.
+  apply Triple_hexists; intros Q1. rewrite hstar_comm; apply Triple_hpure; intros M3.
+  xtpull. simpl. applys Triple_let EA1.
   (* --LATER: typeclass should not be resolved arbitrarily to EA if EA1 is not provided *)
   { rewrite Triple_eq_himpl_Wp. applys* M1. }
   { intros X. rewrite Triple_eq_himpl_Wp.
-    unfold Subst1. rewrite <- isubst_add_eq_subst1_isubst. applys* M2. }
+    unfold Subst1. rewrite <- isubst_add_eq_subst1_isubst. xchange M3. applys* M2. }
 Qed.
+
+(* Lemma Wpgen_sound_let_typed_val : forall v E (C:trm -> trm) `{EA:Enc A} (F2of:A->Formula), *)
+(*   evalctx C -> *)
+(*   (forall V, F2of V ====> @Wpsubst E (C ``V)) -> *)
+(*   Wpgen_let_trm_cont (Wptag (Wpgen_val_unlifted v)) F2of ====> Wp (isubst E (C v)). *)
+(* Proof using. *)
+(*   introv HC M1. intros A1 EA1. applys qimpl_Wp_of_Triple. intros Q. *)
+(*   remove_MkStruct. applys~ Triple_isubst_evalctx EA. *)
+(*   { rewrite Triple_eq_himpl_Wp. lets K: Wpgen_sound_val. *)
+(*     unfold Wpgen_sound in K. simpl in K. xchange K. } *)
+(*   { intros V. rewrite Triple_eq_himpl_Wp. xchange M1. } *)
+(* Qed. *)
 
 Lemma Wpgen_sound_let_typed_val : forall v E (C:trm -> trm) `{EA:Enc A} (F2of:A->Formula),
   evalctx C ->
   (forall V, F2of V ====> @Wpsubst E (C ``V)) ->
-  Wpgen_let_trm_cont (Wptag (Wpgen_val_unlifted v)) F2of ====> Wp (isubst E (C v)).
+  Wpgen_let_trm (Wptag (Wpgen_val_unlifted v)) F2of ====> Wp (isubst E (C v)).
 Proof using.
-  introv HC M1. intros A1 EA1. applys qimpl_Wp_of_Triple. intros Q.
-  remove_MkStruct. applys~ Triple_isubst_evalctx EA.
+  introv HC M1; intros A1 EA1. applys qimpl_Wp_of_Triple; intros Q. remove_MkStruct.
+  apply Triple_hexists; intros Q1.
+  rewrite hstar_comm; apply Triple_hpure; intros M2.
+  applys~ Triple_isubst_evalctx EA.
   { rewrite Triple_eq_himpl_Wp. lets K: Wpgen_sound_val.
     unfold Wpgen_sound in K. simpl in K. xchange K. }
-  { intros V. rewrite Triple_eq_himpl_Wp. xchange M1. }
+  { intros V. rewrite Triple_eq_himpl_Wp. xchange M2. xchange M1. }
 Qed.
 
 Lemma Wpgen_sound_getval_typed : forall E C t1 `{EA:Enc A} (F2of:A->Formula),
@@ -757,11 +788,13 @@ Proof using.
     { intros v Ev. rewrites~ (>> isubst_evalctx_trm_var Ev).
       apply Triple_of_Wp. applys~ Wpgen_sound_let_typed_val. }
     { introv N. remove_MkStruct. xtpull. intros; false. } }
-  asserts_rewrite (Wpaux_getval_typed Wpgen E t1 (@F2of) = Wpgen_let_trm_cont (Wpgen E t1) F2of).
+  asserts_rewrite (Wpaux_getval_typed Wpgen E t1 (@F2of) = Wpgen_let_trm (Wpgen E t1) F2of).
   { destruct t1; auto. { false C2. hnfs*. } }
-  remove_MkStruct. applys~ Triple_isubst_evalctx EA.
+  remove_MkStruct.
+  apply Triple_hexists; intros Q1. rewrite hstar_comm; apply Triple_hpure; intros M3.
+  applys~ Triple_isubst_evalctx EA.
   { apply Triple_of_Wp. applys M1. }
-  { intros V. apply Triple_of_Wp. applys M2. }
+  { intros V. apply Triple_of_Wp. xchange M3. applys M2. }
 Qed.
 
 Lemma Wpgen_sound_if_trm : forall (F0 F1 F2:Formula) E t0 t1 t2,
@@ -770,10 +803,11 @@ Lemma Wpgen_sound_if_trm : forall (F0 F1 F2:Formula) E t0 t1 t2,
   F2 ====> (Wpsubst E t2) ->
   Wpaux_if_trm F0 F1 F2 ====> Wpsubst E (trm_if t0 t1 t2).
 Proof using.
-  introv M0 M1 M2. intros A EA. applys qimpl_Wp_of_Triple. intros Q.
-  remove_MkStruct. xtpull. simpl. applys Triple_if_trm.
+  introv M0 M1 M2. intros A EA. applys qimpl_Wp_of_Triple. intros Q. remove_MkStruct.
+  apply Triple_hexists; intros Q1. rewrite hstar_comm; apply Triple_hpure; intros M3.
+  xtpull. simpl. applys Triple_if_trm.
   { rewrite Triple_eq_himpl_Wp. applys* M0. }
-  { intros b. apply Triple_of_Wp. applys* Wpgen_sound_if_bool'. }
+  { intros b. apply Triple_of_Wp. xchange M3. applys* Wpgen_sound_if_bool'. }
 Qed.
 
 Lemma Wpgen_sound_if : forall t1 t2 t3,
